authentication for basic hash with n tags done.

examples/easycrypt/basic-hash-mult.ec
@@ -1,36 +1,324 @@
+(* Simple modeling of the Basic Hash protocol, multiple tags. *)
+require import AllCore List FSet SmtMap.
+require import Distr DBool.
+require FelTactic.
 
-(* (* Basic Hash protocol, with n+1 tags and one reader. *) *)
-(* module BasicHashN = { *)
-(*   var ks : key list *)
+(* Key space *)
+type key.
 
-(*   (* We always have at least one key. *) *)
-(*   proc init (n : int) : unit = { *)
-(*     var i, x; *)
-(*     i <- 0; *)
-(*     while (i <= n){ *)
-(*       x <$ dkey; *)
-(*       ks <- x :: ks; *)
-(*     } *)
-(*   } *)
+(* Full, lossless and uniform distribution over keys. *)
+op dkey: { key distr |     is_lossless dkey
+                        /\ is_full dkey
+                        /\ is_uniform dkey } as dkey_llfuuni.
 
-(*   proc tag (i : int) : ptxt = { *)
-(*     var k, n, x; *)
-(*     n <$ dnonce; *)
-(*     i <- if (size ks <= i) then 0 else i; *)
-(*     k <- nth witness ks i; *)
-(*     x <- pair n (H k n); *)
-(*     return x; *)
-(*   } *)
+(* Ptxt space *)
+type ptxt.
 
-(*   proc reader (m : ptxt) : bool = { *)
-(*     var i, b, k; *)
-(*     i <- 0; *)
-(*     b <- false; *)
-(*     while (i < size ks){       *)
-(*       k <- nth witness ks i; *)
-(*       b <- b || snd m = H k (fst m); *)
-(*     } *)
-(*     return b; *)
-(*   } *)
-(* }. *)
+(* Lossless and uniform distribution over ptxts (not full). *)
+op dnonce: { ptxt distr |    is_lossless dnonce
+                          /\ is_uniform dnonce } as dnonce_lluni.
 
+(*-----------------------------------------------------------------------*)
+(* multiple PRF *)
+op F : key -> ptxt -> ptxt.
+
+module type PRFs = {
+  proc init (n : int) : unit
+  proc f(i : int, x : ptxt) : ptxt
+  proc check(i : int, x : ptxt, s : ptxt) : bool
+}.
+
+module type PRFs_Oracles = {
+  include PRFs[-init]
+}.
+
+module PRFs = {
+  var ks : key list
+  
+  proc init(n : int) : unit = {
+    var i, k;
+    i <- 0;
+    while (i < n){
+     k <$ dkey;
+     ks <- k :: ks;
+    } 
+  }
+  
+  proc f(i : int, x : ptxt) : ptxt = {
+    var k;
+    i <- if (size ks <= i) then 0 else i;
+    k <- nth witness ks i;
+    return F k x;
+  }
+
+  proc check(i : int, x : ptxt, s : ptxt) = {
+    var k;
+    i <- if (size ks <= i) then 0 else i;
+    k <- nth witness ks i;
+    return (F k x = s);
+  }
+}.
+
+(* Unforgeable multiple RF *)
+(* We assume that: 
+   i) the hash functions are indistinguishable from a lossless and uniform
+   distributions over ptxts (not full).
+   ii) the hash functions are unforgeable.
+   
+   ii) is a consequence of i) whenever the hash function image set is large. *)
+op drf (i : int) : ptxt distr.
+axiom drf_lluni (i : int) : is_lossless (drf i) /\ is_uniform (drf i).
+
+module EUF_RF = {
+  var n : int
+  var m : (int * ptxt, ptxt) fmap
+  
+  proc init(i : int) : unit = {
+    n <- i;
+    m <- empty;
+  }
+  
+  proc f(i : int, x : ptxt) : ptxt = {
+    var r : ptxt;
+    i <- if (n <= i) then 0 else i;
+
+    if ((i,x) \notin m) {
+      r <$ drf i;
+      m.[(i,x)] <- r;
+    }
+    
+    return oget m.[(i,x)];
+  }
+
+  proc check(i : int, x : ptxt, s : ptxt) = {
+    i <- if (n <= i) then 0 else i;
+    return ((i,x) \in m && oget m.[(i,x)] = s);
+  }
+}.
+
+(*-----------------------------------------------------------------------*)
+(* Basic Hash protocol, multiple tags and one reader. *)
+
+op n_tag : int.
+axiom n_tag_p : 0 < n_tag.  (* We have at least one tag. *)
+
+(* Without initialization *)
+module BasicHash0 (H : PRFs_Oracles) = {
+  proc tag (i : int) : ptxt * ptxt = {
+    var n, h;
+    i <- if (n_tag <= i) then 0 else i;
+    n <$ dnonce;
+    h <@ H.f(i,n);
+    return (n, h);
+  }    
+  
+  proc reader (i : int, n h : ptxt) : bool = {    
+    var b;
+    i <- if (n_tag <= i) then 0 else i;
+    b <- H.check(i, n, h);
+    return b;
+  } 
+}.
+
+(* With initialization *)
+module BasicHash (H : PRFs) = {
+  module BH0 = BasicHash0(H)
+  include BH0
+
+  proc init () : unit = { 
+    H.init(n_tag); 
+  }
+}.
+
+(*-----------------------------------------------------------------------*)
+module type BasicHashT = {
+  proc init () : unit
+  proc tag (_ : int) : ptxt * ptxt
+  proc reader (_: int * ptxt * ptxt) : bool
+}.
+
+module type BasicHashT0 = {
+  include BasicHashT[-init]
+}.
+
+(* Basic Hash, multiple tags, with logs. *)
+module Log (BH : BasicHashT) = {
+  var tag_outputs   : (int * ptxt * ptxt) list
+  var reader_forged : (int * ptxt * ptxt) list
+
+  proc init () : unit = { 
+    BH.init ();
+    tag_outputs <- [];
+    reader_forged <- [];
+  }
+
+  proc tag (i : int) : ptxt * ptxt = {
+    var x, y;
+    (x,y) <@ BH.tag (i);
+    i <- if (n_tag <= i) then 0 else i;
+    tag_outputs <- (i,x,y) :: tag_outputs;
+    return (x,y);
+  }    
+
+  proc reader (i : int, x y : ptxt) : bool = {    
+    var b;
+    b <- BH.reader(i,x,y);
+    (* We log messages accepted by the reader that the tag never send. *)
+    i <- if (n_tag <= i) then 0 else i;
+    if (b && ! (mem tag_outputs (i,x,y))){ 
+      reader_forged <- (i,x,y) :: reader_forged;
+    }
+    return b;
+  }    
+}.
+
+(* Adversary against the Basic Hash protocol authentication *)
+module type Adv (BH : BasicHashT0) = {
+  proc a () : unit
+}.
+
+module type BasicHashF (H : PRFs) = {
+  include BasicHashT
+}.
+
+(* Basic Hash protocol authentication game *)
+module AuthGame (Adv : Adv) (BH : BasicHashF) (H : PRFs) = {
+  module BH = Log(BH(H))
+  module Adv = Adv (BH)
+
+  proc main () = {
+    BH.init ();
+    Adv.a();
+    return (exists x, mem Log.reader_forged x );
+  }
+}.
+
+
+(*-----------------------------------------------------------------------*)
+(* Distinguisher against n_tag PRFs. *)
+module type Distinguisher (F : PRFs_Oracles) = {
+  proc distinguish(): bool
+}.
+
+(* Indistinguishability game for unforgeable PRFs. *)
+module EUF_PRF_IND (F : PRFs) (D : Distinguisher) = {
+  proc main(): bool = {
+    var b;
+
+    F.init(n_tag);
+    b <@ D(F).distinguish();
+    return b;
+  }
+}.
+
+(*-----------------------------------------------------------------------*)
+(* In our PRF/RF distinguisher, we must use a slightly different log,
+   which is identical except that it does not initialize the BasicHash
+   protocol. *)
+module AuxLog (BH : BasicHashT0) = {
+  proc init () : unit = { 
+    Log.tag_outputs <- [];
+    Log.reader_forged <- [];
+  }
+
+  proc tag (i : int) : ptxt * ptxt = {
+    var x, y;
+    (x,y) <@ BH.tag (i);
+    i <- if (n_tag <= i) then 0 else i;
+    Log.tag_outputs <- (i,x,y) :: Log.tag_outputs;
+    return (x,y);
+  }    
+
+  proc reader (i : int, x y : ptxt) : bool = {    
+    var b;
+    b <- BH.reader(i,x,y);
+    (* We log messages accepted by the reader that the tag never send. *)
+    i <- if (n_tag <= i) then 0 else i;
+    if (b && ! (mem Log.tag_outputs (i,x,y))){ 
+      Log.reader_forged <- (i,x,y) :: Log.reader_forged;
+    }
+    return b;
+  }    
+}.
+
+module type BasicHashF0 (H : PRFs_Oracles) = {
+  include BasicHashT0
+}.
+
+(* The PRF/RF distinguisher is almost identical to the authentication game,
+   except that it does not initialize the PRF. *)
+module D (A : Adv) (BH : BasicHashF0) (F : PRFs_Oracles) = {
+  module BH = AuxLog(BH(F))
+  module A = A (BH)
+  
+  proc distinguish () = {
+    BH.init();
+    A.a();
+    return (exists x, mem Log.reader_forged x ); 
+  } 
+}.
+
+(*-----------------------------------------------------------------------*)
+(* Given an adversary A against the Authentication Game, we build an
+   an adversary B against the unforgeable PRF H. *)
+
+(* The probability of winning the indistinguishability game against
+   the RF is identical to the authentication game using the RF. *)
+lemma eq_RF &m (A <: Adv {Log, BasicHash, EUF_RF}) : 
+    Pr[AuthGame(A, BasicHash, EUF_RF).main() @ &m : res] =
+    Pr[EUF_PRF_IND(EUF_RF, D(A, BasicHash0)).main() @ &m : res].
+proof.
+  byequiv; auto; proc; inline *; wp; sim; auto. 
+qed.
+
+(* Idem with PRF *)
+lemma eq_PRF &m (A <: Adv {Log, BasicHash, PRFs}) : 
+    Pr[AuthGame(A, BasicHash, PRFs).main() @ &m : res] =
+    Pr[EUF_PRF_IND(PRFs, D(A, BasicHash0)).main() @ &m : res].
+proof.
+  byequiv; auto; proc; inline *; wp; sim; auto. 
+qed.
+
+(* The adversary cannot win the authentication game instantiated
+    with the ideal unforgeable hash function. *)
+lemma res_0 &m (A <: Adv {Log, BasicHash, PRFs, EUF_RF}) : 
+    Pr[AuthGame(A, BasicHash, EUF_RF).main() @ &m : res] = 0%r.
+proof.
+  byphoare; auto. 
+  hoare; proc*; inline *; wp; sp. 
+  call (_: Log.reader_forged = [] /\ EUF_RF.n = n_tag /\
+           forall j x y, (EUF_RF.m.[(j,x)] <> None && oget EUF_RF.m.[(j,x)] = y)
+                          => (j, x, y) \in Log.tag_outputs{hr}); auto.
+
+  (* tag *)
+  + proc; inline *; auto. 
+  seq 6: (#pre /\ x0 = n /\ i1 = i0 /\ i0 = if n_tag <= i then 0 else i); wp.
+   - by rnd; auto; smt (n_tag_p).
+   - case ((i1, x0) \notin EUF_RF.m).
+    * rcondt 1 => //; wp; rnd; auto.
+     move => &hr [[[Hl Hind] [Heq1 [Heq2 Heq3]]] Hin] r H0; 
+     do 2! (split; [ 1 : smt ()]);
+     move => j x y H1.
+     case (i1{hr} = j /\ x0{hr} = x) => Hx. case: Hx => Hj Hx.
+     - left; split => //=. by rewrite -Hj Heq2 Heq3; auto. by smt ().
+     - right. smt.
+    * rcondf 1; auto; move => &hr [[[Hl [Ht Hind]] Heq] Hin].
+      do 2! (split; [ 1 : smt ()]). 
+      move => j x y H1; right; apply Hind; apply H1.
+
+  (* reader *)
+  + proc; inline *; auto => /=.
+  move => &hr [hyp1 hyp2]; split => //. by smt.
+
+  + move => &hr hyp; split => //; do 2! (split; [ 1 : smt ()]). 
+    move => Ht x H; by smt.
+qed.
+
+(* We conclude. *)
+lemma auth0 &m (A <: Adv {Log, BasicHash, PRFs, EUF_RF}) : 
+    Pr[AuthGame(A, BasicHash, PRFs).main() @ &m : res] = 
+      (   Pr[EUF_PRF_IND(PRFs,   D(A, BasicHash0)).main() @ &m : res] 
+        - Pr[EUF_PRF_IND(EUF_RF, D(A, BasicHash0)).main() @ &m : res] ).
+proof.
+  rewrite (eq_PRF &m A) -(eq_RF &m A) (res_0 &m A); by smt ().
+qed.
